updates

intermediate/Veritas.Intermediate.Logs.fst
@@ -1,10 +1,31 @@
 module Veritas.Intermediate.Logs
 
+let lemma_consistent_log_prefix_consistent (#vcfg:_) (init_map: slot_state_map vcfg) (l:logS vcfg) (i:nat{i <= length l}):
+  Lemma (requires (consistent_log init_map l))
+        (ensures (consistent_log init_map (prefix l i))) = admit()
 
+let to_logk (#vcfg:_) (init_map: slot_state_map vcfg) (l:logS vcfg{consistent_log init_map l}): logK = 
+  admit()
 
-let to_logk (#vcfg:_) (tl:thread_id_logS vcfg{consistent_logS tl}): logK
- = admit()
+let lemma_to_logk_length (#vcfg:_) (init_map: slot_state_map vcfg) (l:logS vcfg{consistent_log init_map l}):
+  Lemma (ensures (length (to_logk init_map l) = length l))
+  = admit()
 
+let lemma_all_entries_valid (#vcfg:_) (init_map: slot_state_map vcfg) (l:logS vcfg{consistent_log init_map l}) (i:seq_index l):
+  Lemma (ensures (let l' = prefix l i in
+                  lemma_consistent_log_prefix_consistent init_map l i;
+                  let ssm' = to_slot_state_map init_map l' in
+                  valid_logS_entry ssm' (index l i)))
+  = admit()
+
+let lemma_to_logk_index (#vcfg:_) (init_map: slot_state_map vcfg) (l:logS _{consistent_log init_map l}) (i:seq_index l):
+  Lemma (ensures (let lk = to_logk init_map l in
+                  let l' = prefix l i in
+                  lemma_consistent_log_prefix_consistent init_map l i;
+                  let ssm' = to_slot_state_map init_map l' in
+                  lemma_all_entries_valid init_map l i;
+                  index lk i = to_logK_entry ssm' (index l i)))                  
+  = admit()
 
 (*
 (* Reproducing definitions from Veritas.Verifier.Thread *)
